viper-total-heaps/PredicateRel.thy
@@ -1,0 +1,254 @@
+theory PredicateRel
+  imports InhaleRel
+begin
+
+lemma case_inside:
+  assumes "\<And>x. P x \<Longrightarrow> Q x"
+      and "\<And>x. \<not> P x \<Longrightarrow> Q x"
+    shows "\<And>x. Q x"
+  using assms
+  by blast
+
+lemma inhale_rel_pred_acc_upd_rel:
+  assumes
+    StateRel: "\<And> \<omega> ns. R \<omega> ns \<Longrightarrow>
+                         state_rel_def_same Pr StateCons TyRep Tr
+                           (AuxPred(temp_perm \<mapsto> pred_eq (RealV p))) ctxt \<omega> ns" and
+              "temp_perm \<notin> dom AuxPred" and
+
+    WfTyRep: "wf_ty_repr_bpl TyRep" and
+    MaskVarDefSame: "mask_var_def Tr = mask_var Tr" and
+    TyInterp: "type_interp ctxt = vbpl_absval_ty TyRep" and
+
+    NullConst: "const_repr Tr CNull = nullConst" and
+    MaskVar: "m_bpl = mask_var Tr" and
+    PredLocBpl: "e_ploc_bpl = FunExp ''P'' [] [e_arg_bpl]" and
+
+    MaskUpdateWf: "mask_update_wf TyRep ctxt mask_upd_bpl" and
+    MaskReadWf: "mask_read_wf TyRep ctxt mask_read_bpl" and
+
+    NewPermBpl: "new_perm = (mask_read_bpl (Var m_bpl) (Var nullConst) e_ploc_bpl
+                                  [TConSingle ''PredicateType_P'', TPrim TBool]) \<guillemotleft>Add\<guillemotright> (Var temp_perm)" and
+    MaskUpdateBpl: "m_upd_bpl = mask_upd_bpl (Var m_bpl) (Var nullConst) e_ploc_bpl new_perm
+                                  [TConSingle ''PredicateType_P'', TPrim TBool]" and
+
+    ArgRel: "exp_rel_vpr_bpl
+                (state_rel Pr StateCons TyRep Tr (AuxPred(temp_perm \<mapsto> pred_eq (RealV p))) ctxt)
+                ctxt_vpr ctxt e_arg_vpr e_arg_bpl" and
+
+    PredFunInterp: "fun_interp ctxt ''P'' = Some (lift_fun_bpl (vbpl_absval_ty TyRep) (0, [TConSingle (TRefId TyRep)], TCon (TFieldId TyRep) [TCon ''PredicateType_P'' [], TPrim TBool]) predicate_loc_P)" and
+    PredName: "pred_id = ''P''" and
+    PredLookup: "ViperLang.predicates (program_total ctxt_vpr) pred_id = Some pdecl" and
+    PredTyArgsLookup: "predicate_decl.args pdecl = ty_args" and
+    PredTyArgs: "ty_args = [TRef]"
+
+  shows "rel_general R
+           (state_rel_def_same Pr StateCons TyRep Tr AuxPred ctxt)
+           (\<lambda> \<omega> \<omega>'. inhale_pred_normal_premise ctxt_vpr StateCons pred_id ty_args [e_arg_vpr] e_p_vpr vs p \<omega> \<omega>')
+           (\<lambda> \<omega>. False) P ctxt
+           (BigBlock name ((Assign m_bpl m_upd_bpl) # cs) str tr, cont)
+           (BigBlock name cs str tr, cont)"
+
+  apply (rule rel_intro)
+   prefer 2
+   apply blast
+proof -
+  fix \<omega> ns \<omega>'
+  assume "R \<omega> ns"
+     and *: "inhale_pred_normal_premise ctxt_vpr StateCons pred_id ty_args [e_arg_vpr] e_p_vpr vs p \<omega> \<omega>'"
+
+  hence InitRel: "state_rel_def_same Pr StateCons TyRep Tr
+                                     (AuxPred(temp_perm \<mapsto> pred_eq (RealV p))) ctxt \<omega> ns"
+    using StateRel
+    by blast
+
+  hence InitRel': "state_rel_def_same Pr StateCons TyRep Tr AuxPred ctxt \<omega> ns"
+    apply (rule state_rel_aux_pred_remove[where ?AuxPred="AuxPred(temp_perm \<mapsto> pred_eq (RealV p))" and ?AuxPred'=AuxPred])
+    by (simp add: assms(2) map_le_def)
+
+  from * have "length vs = 1"
+    by (metis One_nat_def add.right_neutral add_Suc_right inhale_pred_normal_premise_def list.size(3) list.size(4) red_pure_exps_total_Some_lengthD)
+  then obtain arg where "vs = [arg]"
+    by (metis One_nat_def Suc_le_eq impossible_Cons length_greater_0_conv list.exhaust list.size(3) n_not_Suc_n)
+  with * have 1: "inhale_pred_normal_premise ctxt_vpr StateCons pred_id ty_args [e_arg_vpr] e_p_vpr [arg] p \<omega> \<omega>'"
+    by fast
+
+  let ?ploc = "(pred_id,[arg])"
+
+  obtain \<phi>_inh where \<omega>':
+    "(p > 0 \<longrightarrow> consistent_external_wrt_ploc ctxt_vpr \<phi>_inh ?ploc (Abs_preal p)) \<and>
+     get_hh_total \<phi>_inh = get_hh_total_full \<omega> \<and>
+     \<omega>' = (if p = 0 then \<omega> else add_to_nm_loc_total_full (inc_mp_loc_total_full \<omega> ?ploc (Abs_preal p)) ?ploc (get_nm_total \<phi>_inh)) \<and>
+     StateCons \<omega>'"
+    using 1[simplified inhale_pred_normal_premise_def inhale_perm_single_pred_def]
+    by (smt (verit, ccfv_threshold) mem_Collect_eq option_fold.simps(1) positive_real_preal pperm_pnone_pgt zero_preal.abs_eq)
+
+  hence mh_same: "get_mh_total_full \<omega> = get_mh_total_full \<omega>'" and
+    mp_rel: "get_mp_total_full \<omega>' = (get_mp_total_full \<omega>)( ?ploc := get_mp_total_full \<omega> ?ploc + Abs_preal p )"
+     apply simp
+    apply (cases "p = 0")
+    using \<omega>' zero_preal_def
+     apply force
+    apply (subgoal_tac "\<omega>' = add_to_nm_loc_total_full (inc_mp_loc_total_full \<omega> ?ploc (Abs_preal p)) ?ploc (get_nm_total \<phi>_inh)")
+     apply simp
+    by (meson \<omega>')
+
+  obtain mb where
+    LookupMask: "lookup_var (var_context ctxt) ns (mask_var Tr) = Some (AbsV (AMask mb))" and
+    LookupMaskTy: "lookup_var_ty (var_context ctxt) (mask_var Tr) = Some (TConSingle (TMaskId TyRep))" and
+    MaskRel: "mask_rel Pr (field_translation Tr) (get_mh_total_full \<omega>) (get_mp_total_full \<omega>) mb"
+    using state_rel_obtain_mask[OF StateRel[OF \<open>R \<omega> ns\<close>]]
+    by blast
+
+  \<comment> \<open>Construct the value of the new permission from the Viper state.\<close>
+  let ?np = "Rep_preal (get_mp_total_full \<omega> (pred_id,[arg])) + p"
+
+  have LookupTempPerm: "lookup_var (var_context ctxt) ns temp_perm = Some (RealV p)"
+    using state_rel_aux_pred_sat_lookup_2[OF StateRel[OF \<open>R \<omega> ns\<close>]]
+    unfolding pred_eq_def
+    by (metis (full_types) fun_upd_same)
+
+  have null_eval: "red_expr_bpl ctxt (Var nullConst) ns (AbsV (ARef Null))"
+    apply (rule red_expr_red_exprs.RedVar)
+    by (metis NullConst StateRel \<open>R \<omega> ns\<close> boogie_const_rel_lookup boogie_const_val.simps(3) state_rel_boogie_const_rel)
+
+  have e_arg_eval: "red_expr_bpl ctxt e_arg_bpl ns (val_rel_vpr_bpl arg)"
+    using ArgRel[simplified exp_rel_vpr_bpl_def exp_rel_vb_single_def]
+    by (metis 1 InitRel inhale_pred_normal_premise_def list.simps(3) nth_Cons_0 red_exp_list_normal_elim)
+
+  have e_arg_type: "get_type (absval_interp_total ctxt_vpr) arg = TRef"
+    using 1[simplified inhale_pred_normal_premise_def vals_well_typed_def PredTyArgs]
+    by blast
+  then obtain arg_bpl where arg_bpl: "val_rel_vpr_bpl arg = AbsV (ARef arg_bpl)"
+    by (metis has_type_get_type has_type_simps(8) val_rel_vpr_bpl.simps(3))
+
+  have ploc_eval: "red_expr_bpl ctxt e_ploc_bpl ns (AbsV (AField (PredSnapshotField (pred_id, [arg]))))"
+    apply (simp add: PredLocBpl)
+    apply (rule red_expr_red_exprs.RedFunOp)
+    using PredFunInterp
+      apply blast
+     apply (rule red_expr_red_exprs.RedExpListCons)
+    using e_arg_eval
+      apply blast
+     apply (rule red_expr_red_exprs.RedExpListNil)
+    apply (simp add: arg_bpl)
+    using arg_bpl PredName e_arg_type has_type_get_type
+    apply (simp add: lift_fun_bpl_def)
+    by force
+
+  have new_perm_eval: "red_expr_bpl ctxt new_perm ns (LitV (LReal ?np))"
+    apply (simp add: NewPermBpl)
+    apply (rule red_expr_red_exprs.RedBinOp[where ?v1.0="LitV (LReal (Rep_preal (get_mp_total_full \<omega> (pred_id,[arg]))))" and ?v2.0="LitV (LReal p)"])
+      apply (rule mask_read_wf_apply[OF MaskReadWf, where ?m=mb and ?r=Null and ?f="PredSnapshotField (pred_id,[arg])"])
+          apply (metis MaskRel mask_rel_def)
+         apply (simp add: LookupMask MaskVar red_expr_red_exprs.RedVar)
+        apply (simp add: null_eval)
+       apply (simp add: ploc_eval)
+      apply force
+     apply (fastforce intro: RedVar LookupTempPerm)
+    by simp
+
+  \<comment> \<open>Construct the new Boogie heap.\<close>
+  let ?mb' = "mb( (Null, PredSnapshotField (pred_id,[arg])) := ?np )"
+
+  have m_upd_bpl_red: "red_expr_bpl ctxt m_upd_bpl ns (AbsV (AMask ?mb'))"
+    apply (subst \<open>m_upd_bpl = _\<close>)
+    apply (rule mask_update_wf_apply[OF MaskUpdateWf])
+        apply (simp add: LookupMask MaskVar red_expr_red_exprs.RedVar)
+       apply (simp add: null_eval)
+      apply (simp add: ploc_eval)
+    using new_perm_eval
+     apply blast
+    by simp
+
+  have "valid_heap_mask (get_mh_total_full \<omega>)"
+    using InitRel state_rel_wf_mask_simple by blast
+
+  have Disj: "disjoint_list [ {heap_var Tr, heap_var_def Tr},
+                              {mask_var Tr, mask_var_def Tr},
+                              ran (var_translation Tr),
+                              ran (field_translation Tr),
+                              range (const_repr Tr), dom AuxPred]"
+    using InitRel' state_rel_disjoint
+    by blast
+
+  show "\<exists>ns'. red_ast_bpl P ctxt
+                ((BigBlock name (Assign m_bpl m_upd_bpl # cs) str tr, cont), Normal ns)
+                ((BigBlock name cs str tr, cont), Normal ns') \<and>
+              state_rel_def_same Pr StateCons TyRep Tr AuxPred ctxt \<omega>' ns'"
+    apply (rule exI, intro conjI)
+     apply (rule red_ast_bpl_one_simple_cmd)
+     apply (rule RedAssign[where ?ty="TConSingle (TMaskId TyRep)" and ?v="AbsV (AMask ?mb')"])
+    using MaskVar StateRel \<open>R \<omega> ns\<close> state_rel_obtain_mask
+       apply blast
+      apply (simp add: TyInterp)
+    using m_upd_bpl_red
+     apply blast
+    apply (simp only: state_rel_def)
+    apply (simp only: state_rel0_def, intro conjI)
+    using state_rel_wf_mask_simple[OF InitRel] \<omega>'
+                    apply (simp, simp)
+    using \<omega>'
+                  apply fastforce
+                 apply (simp add: TyInterp)
+                apply (rule store_rel_stable[where ?\<omega>=\<omega> and ?ns=ns])
+    using InitRel state_rel_store_rel
+                  apply blast
+                 apply (metis 1 inhale_perm_single_pred_store_same inhale_pred_normal_premise_def)
+                apply (metis InitRel MaskVar state_rel_disj_mask_store update_var_other)
+               apply (simp add: Disj)
+              apply (simp, simp, simp)
+           defer defer defer defer
+           apply (metis InitRel MaskVar field_rel_stable mask_var_disjoint state_rel_field_rel state_rel_state_rel0 update_var_other)
+          apply (metis InitRel MaskVar boogie_const_rel_stable mask_var_disjoint state_rel_boogie_const_rel state_rel_state_rel0 update_var_other)
+         defer
+         apply (metis (no_types, lifting) InitRel' MaskVar aux_vars_pred_sat_def domI mask_var_disjoint state_rel_aux_pred_sat_lookup state_rel_state_rel0 update_var_other)
+  proof -
+    let ?ns' = "update_var (var_context ctxt) ns m_bpl
+                  (AbsV (AMask (mb((Null, PredSnapshotField (pred_id, [arg])) :=
+                                   Rep_preal (get_mp_total_full \<omega> (pred_id, [arg])) + p))))"
+
+    \<comment> \<open>Prove \<^const>\<open>heap_var_rel\<close>\<close>
+    show HeapRel: "heap_var_rel Pr (var_context ctxt) TyRep (field_translation Tr) (heap_var Tr) \<omega>' ?ns'"
+      apply (rule heap_var_rel_stable[OF state_rel0_heap_var_rel[OF InitRel[simplified state_rel_def]]])
+       apply (metis 1 inhale_perm_single_pred_heap_same inhale_pred_normal_premise_def)
+      by (metis InitRel MaskVar mask_var_disjoint state_rel_state_rel0 update_var_other)
+
+    \<comment> \<open>Prove \<^const>\<open>mask_var_rel\<close>\<close>
+    show MaskRel: "mask_var_rel Pr (var_context ctxt) TyRep (field_translation Tr) (mask_var Tr) \<omega>' ?ns'"
+      apply (unfold mask_var_rel_def)
+      apply (rule exI[of _ ?mb'])
+      apply (intro conjI)
+        apply (simp add: MaskVar)
+      using LookupMaskTy
+       apply blast
+      apply (unfold mask_rel_def)
+      apply (intro conjI)
+      using MaskRel[simplified mask_rel_def] mh_same
+         apply auto[1]
+        apply (simp add: MaskRel[simplified mask_rel_def])
+      using MaskRel[simplified mask_rel_def]
+       apply (smt (verit, best) 1 MaskRel[simplified mask_rel_def] fun_upd_apply inhale_pred_normal_premise_def is_bounded_field_bpl.simps(1) prod.sel(2))
+      apply (subst \<open>get_mp_total_full \<omega>' = _\<close>)
+      by (metis (no_types, lifting) 1 Abs_preal_inverse MaskRel[simplified mask_rel_def] fun_upd_apply inhale_pred_normal_premise_def mem_Collect_eq plus_preal.rep_eq prod.inject vb_field.simps(2))
+
+    show "heap_var_rel Pr (var_context ctxt) TyRep (field_translation Tr) (heap_var_def Tr) \<omega>' ?ns'"
+      apply (rule heap_var_rel_stable[OF state_rel_heap_var_def_rel[OF InitRel]])
+       apply (metis 1 inhale_perm_single_pred_heap_same inhale_pred_normal_premise_def)
+      by (metis InitRel MaskVar mask_var_disjoint state_rel_state_rel0 update_var_other)
+
+    show MaskRel: "mask_var_rel Pr (var_context ctxt) TyRep (field_translation Tr) (mask_var_def Tr) \<omega>' ?ns'"
+      apply (subst MaskVarDefSame)
+      using MaskRel
+      by blast
+
+    show "state_well_typed (type_interp ctxt) (var_context ctxt) [] ?ns'"
+      apply (rule state_well_typed_upd_2)
+      using InitRel state_rel_state_well_typed
+       apply blast
+      by (simp add: TyInterp LookupMaskTy MaskVar)
+  qed
+qed
+
+
+end
