viper-total-heaps/TotalStateProperties.thy
@@ -233,6 +233,18 @@ lemma upd_nm_loc_opt_nm__mp_rel [simp]:
   shows "get_mp_nm (upd_nm_loc_opt_nm nm lp nm') = get_mp_nm nm"
   by (cases nm, fastforce)
 
+lemma inc_mp_loc_nm__mh_rel [simp]:
+  shows "get_mh_nm (inc_mp_loc_nm nm lp p) = get_mh_nm nm"
+  by (cases nm, fastforce)
+
+lemma inc_mp_loc_nm__mp_rel [simp]:
+  shows "get_mp_nm (inc_mp_loc_nm nm lp p) = (get_mp_nm nm)( lp := get_mp_nm nm lp + p )"
+  by (cases nm, fastforce)
+
+lemma inc_mp_loc_nm__fnm_rel [simp]:
+  shows "get_fnm_nm (inc_mp_loc_nm nm lp p) = get_fnm_nm nm"
+  by (cases nm, fastforce)
+
 lemma add_to_nm_loc_nm__mh_rel [simp]:
   shows "get_mh_nm (add_to_nm_loc_nm nm lp nm') = get_mh_nm nm"
   by (cases nm, fastforce)
